# Reading Nielsen and Chuang: Chapter 6

I just finished reading Chapter 6 of *Quantum Computation and Quantum Information* by Nielsen and Chuang. 

## Navigation

* [The quantum search algorithm](#the-quantum-search-algorithm)
* [Quantum search as a quantum simulation](#quantum-search-as-a-quantum-simulation)
* [Quantum counting](#quantum-counting)
* [Speeding up the solution of NP-complete problems](#speeding-up-the-solution-of-np-complete-problems)
* [Quantum search of an unstructured database](#quantum-search-of-an-unstructured-database)
* [Optimality of the search algorithm](#optimality-of-the-search-algorithm)
* [Black box algorithm limits](#black-box-algorithm-limits)
* [Chapter problems](#chapter-problems)



## The quantum search algorithm

### The quantum search algorithm - Key Concepts


| Concept                              | Book Section              | Notes                                                                                                  |
|--------------------------------------|---------------------------|--------------------------------------------------------------------------------------------------------|
| Grover iteration                     | 6.1.2                     | (1) Apply the oracle $O$. <br> (2) Apply the Hadamard transform $H^{\otimes n}$. <br> (3) Perform a conditional phase shift on the computer, with every computation basis state except $\ket{0}$ recieving a phase shift of -1, $\ket{x}\rightarrow -(-1)^{\delta_{x0}}\ket{x}$. <br> (4) Apply the Hadamard transform $H^{\otimes n}$. <br> $G=(2\ket{\psi}\bra{\psi}-I)O$, where $\ket{\psi}$ is the equally weighted superposition of states. |



### The quantum search algorithm - Exercises

**Exercise 6.1**

Show that the unitary operator corresponding to the phase shift in the Grover iteration is $2\ket{0}\bra{0} - I$.

<details style="margin-bottom: 20px;" markdown="1">
<summary>Solution</summary>

Let's calculate $U\ket{x}$ and compare results to desired behavior, where $U=2\ket{0}\bra{0}-I$.

$$\begin{aligned}
U\ket{x} &= \left(2\ket{0}\bra{0} - I\right)\ket{x} \\
&= 2\ket{0}\braket{0\vert x} - \ket{x} \\
&= 2\delta_{x0}\ket{0} - \ket{x} \\
&= -(-1)^{\delta_{x0}}\ket{x}
\end{aligned}$$

This matches the desired behavior and so the unitary operator corresponding to the phase shift in the Grover iteration is $2\ket{0}\bra{0} - I$.

</details>


**Exercise 6.2**

Show that the operation $(2\ket{\psi}\bra{\psi}-I)$ applied to a general state $\sum_{k}\alpha_k\ket{k}$ produces

$$\begin{aligned}
\sum_{k}\lbrack -\alpha_k+2\braket{\alpha}\rbrack\ket{k},
\end{aligned}$$

where $\braket{\alpha}\equiv \sum_k\alpha_k/N$ is the mean value of the $\alpha_k$. For this reason, $(2\ket{\psi}\bra{\psi}-I)$ is sometimes referred to as the inversion about mean operation.

<details style="margin-bottom: 20px;" markdown="1">
<summary>Solution</summary>

First let's rewrite $\ket{\psi}\bra{\psi}$ using equation 6.4

$$\begin{aligned}
\ket{\psi}\bra{\psi} &= \frac{1}{N}\sum_{x=0}^{N-1}\sum_{x'=0}^{N-1} \ket{x}\bra{x'}
\end{aligned}$$

Now let's use this in the exercise

$$\begin{aligned}
(2\ket{\psi}\bra{\psi}-I)\sum_{k}\alpha_k\ket{k} &= \sum_{k}2\alpha_k\ket{\psi}\braket{\psi\vert k}-\alpha_k\ket{k}\\
&= \sum_{k}\left(\sum_{x=0}^{N-1}\sum_{x'=0}^{N-1} \frac{2\alpha_k}{N}\ket{x}\braket{x'\vert k}\right)-\alpha_k\ket{k}\\
&= \sum_{k}\left(\sum_{x=0}^{N-1}\sum_{x'=0}^{N-1} \frac{2\alpha_k}{N}\ket{x} \delta_{kx'}\right)-\alpha_k\ket{k}\\
&= \sum_{k}\left(\sum_{x=0}^{N-1} \frac{2\alpha_k}{N}\ket{x}\right) -\alpha_k\ket{k}\\
&= \left(\sum_{x=0}^{N-1} \left(\sum_{k}\frac{2\alpha_k}{N}\right)\ket{x}\right) - \left(\sum_{k}\alpha_k\ket{k}\right)\\
&= \left(\sum_{x=0}^{N-1}2\braket{\alpha}\ket{x}\right) - \left(\sum_{k}\alpha_k\ket{k}\right)\\
&= \sum_{k}2\braket{\alpha}\ket{k} - \alpha_k\ket{k} & \text{relable $x$ as $k$}\\
&= \sum_{k}\lbrack 2\braket{\alpha} - \alpha_k\rbrack\ket{k} \\
\end{aligned}$$

</details>


**Exercise 6.3**


















